\section{Definition of RVSI}

\input{sections/si}

%%%%%%%%%%%%%%%
\begin{frame}{Principle of \rvsi{}}
  \begin{itemize}
    \setlength{\itemsep}{10pt}
    \item<1-> Parameters ($k_1, k_2, k_3$) to control the severity of the anomalies w.r.t SI
    \item<2-> $\rc{}~\footnotemark \supset \rvsi(k_1, k_2, k_3) \supset \si{}$
    \item<2-> $\rvsi(\infty,\infty,\infty) = \rc \qquad \rvsi(1,0,\ast) = \si$
  \end{itemize}
  \footnotetext{RC: Read Committed}
\end{frame}
%%%%%%%%%%%%%%%

%%%%%%%%%%%%%%%
\begin{frame}{Principle of \rvsi{}}
  \begin{quote}
    $\ldots$\\
    \hfill -- ``Snapshot Read'' property of SI
  \end{quote}

  \begin{enumerate}[<+->]
    \setlength{\itemsep}{10pt}
    \item ``stale'' data versions		\hfill \uncover<4->{\red{bounded staleness}}
    \item ``concurrent'' data versions  	\hfill \uncover<5->{\red{bounded concurrency level}}
    \item ``non-snapshot'' data versions	\hfill \uncover<6->{\red{bounded distance}}
  \end{enumerate}
\end{frame}
%%%%%%%%%%%%%%%

%%%%%%%%%%%%%%%
\begin{frame}{Illustration of RVSI}
  \fignocaption{width = 0.85\textwidth}{figs/rvsi-definition.pdf}
\end{frame}
%%%%%%%%%%%%%%%

%%%%%%%%%%%%%%%
\begin{frame}{Definition of RVSI}
  \begin{align*}
    & \red{(\konebv{})} \\
    \forall r_i(x_{j}), w_k(x_k), c_k \in h: 
    & \left(c_j \in h \land \bigwedge_{k=1}^{m} \left(c_j \hp c_k \hp s_i \right)\right) \Rightarrow m < k_1, \\[10pt]
    & \red{(\ktwofv{})} \\
    \forall r_i(x_{j}), w_k(x_k), c_k \in h:
    & \left(c_j \in h \land \bigwedge_{k=1}^{m} \left(s_i \hp c_k \hp c_j \right)\right) \Rightarrow m \le k_2, \\[10pt]
    & \red{(\kthreesv{})} \\
    \forall r_i(x_j), r_i(y_l), w_k(x_k), c_k \in h:
    & \left(\bigwedge_{k=1}^{m} \left(c_j \hp c_k \hp c_l \right)\right) \Rightarrow m \le k_3.
  \end{align*}
\end{frame}
%%%%%%%%%%%%%%%

%%%%%%%%%%%%%%%
\begin{frame}{Definition of \rvsi{}}
  \begin{equation*}
    h \in \rvsi{} \iff h \in \konebv{} \cap \ktwofv{} \cap \kthreesv{} \cap \wcf{}.
  \end{equation*}

  \vspace{0.50cm}
  \begin{theorem}
    \[
      \emph{\rvsi}(1,0,\ast) = \emph{\si}.
    \]
  \end{theorem}
\end{frame}
%%%%%%%%%%%%%%%

%%%%%%%%%%%%%%%
\begin{frame}{}
\end{frame}
%%%%%%%%%%%%%%%

%%%%%%%%%%%%%%%
\begin{frame}{}
\end{frame}
%%%%%%%%%%%%%%%
